Test/floats/Havoc.bpl
@@ -4,15 +4,15 @@
 function {:builtin "(_ to_fp 11 53) RNE"} TO_FLOAT64_REAL(real) returns (float53e11);
 
 procedure double_range_true() returns () {
-	var x : float53e11;
-	havoc x;
-	if (x >= TO_FLOAT64_REAL(-1e307) && x <= TO_FLOAT64_REAL(1e307)) {	
-		assert(x==x);
-	}
+  var x : float53e11;
+  havoc x;
+  if (x >= TO_FLOAT64_REAL(-1e307) && x <= TO_FLOAT64_REAL(1e307)) {  
+    assert(x==x);
+  }
 }
 
 procedure double_range_false() returns () {
-	var x : float53e11;
-	havoc x;
-	assert(x==x);
+  var x : float53e11;
+  havoc x;
+  assert(x==x);
 }
