Test/floats/IncorrectTypeConv.bpl
@@ -9,15 +9,15 @@ function {:builtin "(_ to_fp 8 23) RNE"} TO_FLOAT823_FLOAT824(float24e8) returns
 function {:builtin "(_ to_fp 8 24) RNE"} TO_FLOAT824_FLOAT823(float23e8) returns (float24e8);
 
 procedure foo(x : float24e8) returns (r : float24e8) {
-	r := TO_FLOAT823_INT(5); // Error
-	r := TO_FLOAT823_REAL(5.0); // Error
-	r := TO_FLOAT823_BV31(0bv31); // Error
-	r := TO_FLOAT823_BV32(0bv32); // Error
-	r := TO_FLOAT823_FLOAT824(0e0f24e8); // Error
-	r := TO_FLOAT824_FLOAT823(0e0f23e8); // Error
-	
-	r := TO_FLOAT823_FLOAT824(x); // Error
-	r := TO_FLOAT824_FLOAT823(x); // Error
-	
-	return;
+  r := TO_FLOAT823_INT(5); // Error
+  r := TO_FLOAT823_REAL(5.0); // Error
+  r := TO_FLOAT823_BV31(0bv31); // Error
+  r := TO_FLOAT823_BV32(0bv32); // Error
+  r := TO_FLOAT823_FLOAT824(0e0f24e8); // Error
+  r := TO_FLOAT824_FLOAT823(0e0f23e8); // Error
+  
+  r := TO_FLOAT823_FLOAT824(x); // Error
+  r := TO_FLOAT824_FLOAT823(x); // Error
+  
+  return;
 }
